implementation/repl_funScript.sml
@@ -1,19 +1,11 @@
 open HolKernel boolLib bossLib lcsymtacs
-open lexer_funTheory mmlParseTheory AstTheory inferTheory CompilerTheory PrinterTheory compilerTerminationTheory bytecodeEvalTheory replTheory
+open lexer_implTheory mmlParseTheory AstTheory inferTheory CompilerTheory
+     PrinterTheory compilerTerminationTheory bytecodeEvalTheory replTheory
 
 val _ = new_theory "repl_fun";
 
-val lex_chunk_def = Define `
-  lex_chunk input = SOME (lexer_fun input, "")`; (* ugly hack, needs doing properly *)
-
-(* EVAL ``parse(  lexer_fun "val b = 5;val a = 7")`` *)
-
-val lex_chunk_thm = prove(
-  ``(lex_chunk input = SOME (ts,rest)) ==> LENGTH rest < LENGTH input``,
-  cheat);
-
 val _ = Hol_datatype`repl_fun_state = <|
-  rtype_bindings : typeN list ; rctors : ctor_env ; rbindings : binding_env;
+  rtypes : typeN list ; rctors : ctor_env ; rbindings : binding_env;
   rmenv : (modN, (varN,num#infer_t) env) env ; rcenv : tenvC;
   rtenv : (tvarN,num#infer_t) env ;
   rcompiler_state : compiler_state ;
@@ -30,17 +22,19 @@ val init_bc_state_def =  Define`
 
 val init_repl_fun_state = Define`
   init_repl_fun_state = <|
-    rtype_bindings := []; rctors := []; rbindings := [];
+    rtypes := []; rctors := []; rbindings := [];
     rmenv := []; rcenv := []; rtenv := [];
     rcompiler_state := init_compiler_state ; decs := [] |>`
 
 val print_result_def = Define `
   print_result s bs =
-    simple_printer (FLAT (MAP (preprint_dec s.rcompiler_state) s.decs)) (cpam s.rcompiler_state) bs.stack`
+    simple_printer
+      (FLAT (MAP (preprint_dec s.rcompiler_state) s.decs))
+      (cpam s.rcompiler_state) bs.stack`
 
 val update_state_def = Define`
   update_state s tbs cts bds (rm,rc,rt) cs ds =
-  s with <| rtype_bindings  := tbs ++ s.rtype_bindings
+  s with <| rtypes  := tbs ++ s.rtypes
           ; rctors          := cts ++ s.rctors
           ; rbindings       := bds ++ s.rbindings
           ; rmenv           := rm ++ s.rmenv
@@ -65,7 +59,7 @@ val parse_elaborate_typecheck_compile_def = Define `
       NONE => Failure "parse error"
     | (* case: ast_prog produced *)
       SOME ast_prog =>
-        let (ts,cts,bds,prog) = elab_prog s.rtype_bindings s.rctors s.rbindings ast_prog in
+        let (ts,cts,bds,prog) = elab_prog s.rtypes s.rctors s.rbindings ast_prog in
           case FST (infer_prog s.rmenv s.rcenv s.rtenv prog init_infer_state) of
             (* type inference failed to find type *)
           | Failure _ => Failure "type error"
@@ -79,9 +73,12 @@ val install_code_def = Define `
     bs with <| code := bs.code ++ code ;
                pc := next_addr bs.inst_length bs.code |>`;
 
+val tac = (WF_REL_TAC `measure (LENGTH o SND)` THEN REPEAT STRIP_TAC
+           THEN IMP_RES_TAC lex_until_toplevel_semicolon_LESS);
+
 val main_loop_def = tDefine "main_loop" `
   main_loop (bs,s) input =
-    case lex_chunk input of
+    case lex_until_toplevel_semicolon input of
       (* case: nothing but white space found, i.e. end of input *)
       NONE => Terminate
     | (* case: tokens have been read, now eval-print-and-loop *)
@@ -96,10 +93,7 @@ val main_loop_def = tDefine "main_loop" `
               NONE => Diverge
             | (* case: evaluation terminated, print result and continue *)
               SOME new_bs => Result (print_result new_s new_bs)
-                                    (main_loop (new_bs,new_s) rest_of_input)
-`
-  (WF_REL_TAC `measure (LENGTH o SND)` THEN REPEAT STRIP_TAC
-   THEN IMP_RES_TAC lex_chunk_thm)  ;
+                                    (main_loop (new_bs,new_s) rest_of_input) ` tac ;
 
 val repl_fun_def = Define`
   repl_fun input = main_loop (init_bc_state,init_repl_fun_state) input`;
@@ -116,11 +110,11 @@ val _ = computeLib.add_funs [lemma1,lemma2]
 
 val input = ``"val x = 1"``
 
-val tokens = EVAL ``lex_chunk ^input`` |> concl |> rhs |> rand |> rator |> rand
+val tokens = EVAL ``lex_until_toplevel_semicolon ^input`` |> concl |> rhs |> rand |> rator |> rand
 val ast_prog = EVAL ``parse ^tokens`` |> concl |> rhs |> rand
 val s = ``init_repl_fun_state``
 
-val prog = EVAL ``elab_prog ^s.rtype_bindings ^s.rctors ^s.rbindings ^ast_prog``
+val prog = EVAL ``elab_prog ^s.rtypes ^s.rctors ^s.rbindings ^ast_prog``
   |> concl |> rhs |> rand |> rand |> rand
 
 val res = EVAL ``FST (infer_prog ^s.rmenv ^s.rcenv ^s.rtenv ^prog init_infer_state)``
@@ -142,18 +136,6 @@ TODO:
    should really be something like:
 
      Failure error_msg => Error error_msg (main_loop (bs,s) rest_of_input)
-
- - Printer function should have a very simple interface at least
-   internally. Example:
-
-     val (x,y,z) = (5,Nil,7);
-
-   should call [(0,"x");(1,"y");(2,"z")] and [(7,"Nil")] a special
-   function at the end. This function produces:
-
-     val x = 5
-     val y = Nil
-     val z = 7
 
 *)
 
