parsing/lexer_implScript.sml
@@ -1,0 +1,64 @@
+
+open HolKernel Parse boolLib bossLib;
+
+val _ = new_theory "lexer_impl";
+
+open stringTheory stringLib listTheory TokensTheory lexer_funTheory;
+
+val _ = Hol_datatype`semihider = SH_END | SH_PAR`
+(* extend with SH_BRACE and SH_BRACKET when records and lists
+   are part of the syntax *)
+
+val lex_aux_def = tDefine "lex_aux" `
+  lex_aux acc error stk input =
+    case next_token input of
+    | (* case: end of input, only white space found *)
+      NONE => NONE
+    | (* case: token found *)
+      SOME (token, rest) =>
+        if token = SemicolonT /\ (stk = [] \/ error) then SOME (REVERSE acc, rest)
+        else
+          let new_acc = (token::acc) in
+            if error then lex_aux new_acc error stk rest
+            else if token = LetT then lex_aux new_acc F (SH_END::stk) rest
+            else if token = StructT then lex_aux new_acc F (SH_END::stk) rest
+            else if token = SigT then lex_aux new_acc F (SH_END::stk) rest
+            else if token = LparT then lex_aux new_acc F (SH_PAR::stk) rest
+            else if token = EndT then
+              case stk of
+                  SH_END :: stk' => lex_aux new_acc F stk' rest
+                | _ => lex_aux new_acc T [] rest
+            else if token = RparT then
+              case stk of
+                  SH_PAR :: stk' => lex_aux new_acc F stk' rest
+                | _ => lex_aux new_acc T [] rest
+            else lex_aux new_acc F stk rest `
+  (WF_REL_TAC `measure (LENGTH o SND o SND o SND)`
+   THEN SRW_TAC []  [next_token_LESS]);
+
+val lex_until_toplevel_semicolon_def = Define `
+  lex_until_toplevel_semicolon input = lex_aux [] F [] input`;
+
+val lex_aux_LESS = prove(
+  ``!acc error stk input.
+      (lex_aux acc error stk input = SOME (ts, rest)) ==>
+      LENGTH rest < LENGTH input``,
+  HO_MATCH_MP_TAC (fetch "-" "lex_aux_ind")
+  THEN REPEAT STRIP_TAC THEN POP_ASSUM MP_TAC
+  THEN ONCE_REWRITE_TAC [lex_aux_def]
+  THEN Cases_on `next_token input` THEN FULL_SIMP_TAC (srw_ss()) []
+  THEN Cases_on `x` THEN FULL_SIMP_TAC (srw_ss()) [LET_DEF]
+  THEN SRW_TAC [] [] THEN IMP_RES_TAC next_token_LESS
+  THEN FULL_SIMP_TAC std_ss [] THEN RES_TAC
+  THEN IMP_RES_TAC arithmeticTheory.LESS_TRANS
+  THEN Cases_on `stk` THEN FULL_SIMP_TAC (srw_ss()) []
+  THEN Cases_on `h` THEN FULL_SIMP_TAC (srw_ss()) []);
+
+val lex_until_toplevel_semicolon_LESS = store_thm(
+  "lex_until_toplevel_semicolon_LESS",
+  ``(lex_until_toplevel_semicolon input = SOME (ts,rest)) ==>
+    LENGTH rest < LENGTH input``,
+  SIMP_TAC std_ss [lex_until_toplevel_semicolon_def]
+  THEN REPEAT STRIP_TAC THEN IMP_RES_TAC lex_aux_LESS);
+
+val _ = export_theory();
